WIP: Rename Induction.Data to Induction.Context

Lean4Axiomatic/Integer/Impl/Difference/Induction.lean
@@ -14,25 +14,26 @@ variable {ℕ : Type} [Natural ℕ]
 
 /-- TODO -/
 theorem sub_eqv_diff
-    {n m : ℕ} : (n:Difference ℕ) - (m:Difference ℕ) ≃ n——m
+    {n m : ℕ} : (n:Difference ℕ) - m ≃ n——m
     := calc
-  _ = (n:Difference ℕ) - (m:Difference ℕ) := rfl
-  _ = (n——0) - (m——0)                     := rfl
-  _ ≃ (n——0) + -(m——0)                    := sub_defn
-  _ = (n——0) + (0——m)                     := rfl
-  _ = (n + 0)——(0 + m)                    := rfl
-  _ ≃ n——(0 + m)                          := diff_substL AA.identR
-  _ ≃ n——m                                := diff_substR AA.identL
+  _ = (n:Difference ℕ) - m := rfl
+  _ = (n——0) - (m——0)      := rfl
+  _ ≃ (n——0) + -(m——0)     := sub_defn
+  _ = (n——0) + (0——m)      := rfl
+  _ = (n + 0)——(0 + m)     := rfl
+  _ ≃ n——(0 + m)           := diff_substL AA.identR
+  _ ≃ n——m                 := diff_substR AA.identL
 
 /-- TODO -/
 def ind_diff
     {motive : Difference ℕ → Sort u} [IndexedFamily motive]
-    (d : Induction.Data motive)
+    (ctx : Induction.Context motive)
     : (a : Difference ℕ) → motive a
     := by
   intro (n——m)
   show motive (n——m)
-  have : motive (n - m) := d.on_diff n m
+  -- TODO: `ind_diff` only needs `on_diff` from `Context` -- maybe `Ctx.Ops`?
+  have : motive (n - m) := ctx.on_diff n m
   have : motive (n——m) := fsubst sub_eqv_diff this
   exact this
 
@@ -43,53 +44,54 @@ local instance ind_ops : Induction.Ops (Difference ℕ) := {
 /-- TODO -/
 theorem ind_diff_subst
     {motive : Difference ℕ → Sort u} [IndexedFamily motive]
-    (d : Induction.Data motive) {a₁ a₂ : Difference ℕ} (a_eqv : a₁ ≃ a₂)
-    : fsubst ‹a₁ ≃ a₂› (d.ind_diff a₁) ≃ d.ind_diff a₂
+    (ctx : Induction.Context motive) {a₁ a₂ : Difference ℕ} (a_eqv : a₁ ≃ a₂)
+    : fsubst ‹a₁ ≃ a₂› (ctx.ind_diff a₁) ≃ ctx.ind_diff a₂
     := by
   revert a₁ a₂; intro (n₁——m₁) (n₂——m₂) (_ : n₁——m₁ ≃ n₂——m₂)
   let a₁ := n₁——m₁; let a₂ := n₂——m₂
-  let od₁ := d.on_diff n₁ m₁; let od₂ := d.on_diff n₂ m₂
-  let idod := d.ind_diff
-  show fsubst ‹a₁ ≃ a₂› (d.ind_diff a₁) ≃ d.ind_diff a₂
+  let od₁ := ctx.on_diff n₁ m₁; let od₂ := ctx.on_diff n₂ m₂
+  show fsubst ‹a₁ ≃ a₂› (ctx.ind_diff a₁) ≃ ctx.ind_diff a₂
   have diff_eqv : (n₂:Difference ℕ) - m₂ ≃ n₁ - m₁ := calc
     _ = (n₂:Difference ℕ) - m₂ := rfl
     _ ≃ n₂——m₂                 := sub_eqv_diff
     _ ≃ n₁——m₁                 := Rel.symm ‹n₁——m₁ ≃ n₂——m₂›
     _ ≃ n₁ - m₁                := Rel.symm sub_eqv_diff
   calc
-    _ = fsubst ‹a₁ ≃ a₂› (idod a₁)
+    _ = fsubst ‹a₁ ≃ a₂› (ctx.ind_diff a₁)
       := rfl
     _ = fsubst ‹a₁ ≃ a₂› (fsubst sub_eqv_diff od₁)
       := rfl
     _ ≃ fsubst (Rel.trans sub_eqv_diff ‹a₁ ≃ a₂›) od₁
       := fsubst_trans
     _ ≃ fsubst (Rel.trans sub_eqv_diff ‹a₁ ≃ a₂›) (fsubst diff_eqv od₂)
-      := fsubst_substR (Rel.symm d.on_diff_subst)
+    -- TODO: Needs `on_diff` and `on_diff_subst` from `Context`
+      := fsubst_substR (Rel.symm ctx.on_diff_subst)
     _ ≃ fsubst (Rel.trans diff_eqv (Rel.trans sub_eqv_diff ‹a₁ ≃ a₂›)) od₂
       := fsubst_trans
     _ = fsubst (sub_eqv_diff (ℕ := ℕ)) od₂
       := rfl
-    _ = idod a₂
+    _ = ctx.ind_diff a₂
       := rfl
 
 /-- TODO -/
 theorem ind_diff_eval
     {motive : Difference ℕ → Sort u} [IndexedFamily motive]
-    (d : Induction.Data motive) {n m : ℕ}
-    : d.ind_diff (n - m) ≃ d.on_diff n m
+    (ctx : Induction.Context motive) {n m : ℕ}
+    : ctx.ind_diff (n - m) ≃ ctx.on_diff n m
     := by
   calc
-    _ = d.ind_diff (n - m)
+    _ = ctx.ind_diff (n - m)
         := rfl
-    _ ≃ fsubst (Rel.symm sub_eqv_diff) (d.ind_diff (n——m))
-        := Rel.symm (ind_diff_subst d (Rel.symm sub_eqv_diff))
-    _ = fsubst (Rel.symm (sub_eqv_diff (ℕ := ℕ))) (fsubst sub_eqv_diff (d.on_diff n m))
+    _ ≃ fsubst (Rel.symm sub_eqv_diff) (ctx.ind_diff (n——m))
+    -- TODO: Needs `ind_diff_subst`, so needs all of `Context`
+        := Rel.symm (ind_diff_subst ctx (Rel.symm sub_eqv_diff))
+    _ = fsubst (Rel.symm (sub_eqv_diff (ℕ := ℕ))) (fsubst sub_eqv_diff (ctx.on_diff n m))
         := rfl
-    _ ≃ fsubst (Rel.trans sub_eqv_diff (Rel.symm sub_eqv_diff)) (d.on_diff n m)
+    _ ≃ fsubst (Rel.trans sub_eqv_diff (Rel.symm sub_eqv_diff)) (ctx.on_diff n m)
         := fsubst_trans
-    _ = fsubst Rel.refl (d.on_diff n m)
+    _ = fsubst Rel.refl (ctx.on_diff n m)
         := rfl
-    _ ≃ d.on_diff n m
+    _ ≃ ctx.on_diff n m
         := fsubst_refl
 
 def ind_props : Induction.Props (Difference ℕ) := {
