Lean4Axiomatic/Rational/Exponentiation.lean
@@ -274,7 +274,7 @@ theorem pow_substL
       _ ≃ p₂^n / p₁^m        := div_substL (Natural.pow_substL ‹p₁ ≃ p₂›)
       _ ≃ p₂^n / p₂^m        := div_substR (Natural.pow_substL ‹p₁ ≃ p₂›)
       _ ≃ p₂^((n:ℤ) - (m:ℤ)) := eqv_symm Integer.pow_diff
-  let ind_ctx := Integer.ind_constraints_prop on_diff
+  let ind_ctx := Integer.ind_context_prop on_diff
 
   have : motive a := ind_ctx.ind_diff a
   have : p₁^a ≃ p₂^a := this
@@ -301,7 +301,7 @@ theorem pow_preserves_nonzero {p : ℚ} {a : ℤ} [AP (p ≄ 0)] : p^a ≄ 0 := 
     have : p^n ≃ 0 := div_eqv_0.mp this
     have : p^n ≄ 0 := Natural.pow_preserves_nonzero_base ‹AP (p ≄ 0)›.ev
     exact absurd ‹p^n ≃ 0› ‹p^n ≄ 0›
-  let ind_ctx := Integer.ind_constraints_prop on_diff
+  let ind_ctx := Integer.ind_context_prop on_diff
 
   have : motive a := ind_ctx.ind_diff a
   have : p^a ≄ 0 := this
